theories/Labelled_Transition_System/Definitions/Termination.v
@@ -25,7 +25,7 @@
 
 From Stdlib.Unicode Require Import Utf8.
 From stdpp Require Import base countable.
-From Must Require Import gLts Bisimulation Lts_OBA.
+From Must Require Import gLts Bisimulation Lts_OBA MultisetHelper.
 
 
 (******************************************** Termination ***************************************************)
